Parikh/Pilling.thy
@@ -578,10 +578,10 @@ proof -
     case True
     from * finite_Nts exists_mapping obtain \<gamma> \<gamma>' where **: "mapping_Nt_Var (Nts P) \<gamma> \<gamma>'" by metis
 
-    let ?sol = "\<lambda>i. if i < card (Nts P) then CFL.Lang P (\<gamma> i) else {}"
+    let ?sol = "\<lambda>i. if i < card (Nts P) then Lang_lfp P (\<gamma> i) else {}"
     from ** True have "\<gamma>' S < card (Nts P)" "\<gamma> (\<gamma>' S) = S"
       unfolding mapping_Nt_Var_def bij_betw_def by auto
-    with CFL_Lang_eq_CFG_Lang have ***: "Lang P S = ?sol (\<gamma>' S)" by metis
+    with Lang_lfp_eq_Lang have ***: "Lang P S = ?sol (\<gamma>' S)" by metis
 
     from * ** CFG_eq_sys.CFL_is_min_sol obtain sys
       where sys_intro: "(\<forall>eq \<in> set sys. regular_fun eq) \<and> (\<forall>eq \<in> set sys. \<forall>x \<in> vars eq. x < length sys)
